Launchbury/ArityCorrectSestoft.thy
@@ -1,0 +1,72 @@
+theory ArityCorrectSestoft
+imports ArityCorrect SestoftCorrect
+begin
+
+fun stack_arity :: "stack \<Rightarrow> Arity"
+  where "stack_arity [] = 0"
+      | "stack_arity (Arg x # S) = inc_Arity (stack_arity S)"
+      | "stack_arity (Upd x # S) = stack_arity S"
+      | "stack_arity (Dummy x # S) = stack_arity S"
+
+nominal_function maybeVar :: "exp \<Rightarrow> var option" where
+  "maybeVar (Var x) = Some x" |
+  "maybeVar (Lam [x]. e) = None" |
+  "maybeVar (App e x) = None" |
+  "maybeVar (Let as e) = None"
+  unfolding maybeVar_graph_aux_def eqvt_def
+  apply simp
+  apply simp
+  apply (metis exp_strong_exhaust)
+  apply auto
+  done
+nominal_termination (eqvt) by lexicographic_order
+
+fun conf_arities :: "conf \<Rightarrow> AEnv"
+  where "conf_arities (\<Gamma>,e,S) = (case maybeVar e of Some x \<Rightarrow> AE_singleton x \<cdot> (up\<cdot>(stack_arity S)) | None \<Rightarrow> \<bottom>)"
+
+fun trace_arities :: "conf list \<Rightarrow> AEnv"
+  where
+  "trace_arities [] = \<bottom>"
+ |"trace_arities ((\<Gamma>,e,S)#T) = conf_arities (\<Gamma>,e,S) \<squnion> trace_arities T"
+
+
+context CorrectArityAnalysis
+begin
+
+lemma arity_preservation:
+  assumes "(\<Gamma>, e, S) \<Rightarrow> (\<Gamma>', e', S')"
+  shows "Afix \<Gamma>'\<cdot>(Aexp e'\<cdot>(stack_arity S')) \<sqsubseteq> Afix \<Gamma>\<cdot>(Aexp e\<cdot>(stack_arity S))" sorry
+
+lemma arity_correct_now:
+  shows "conf_arities (\<Gamma>, e, S) \<sqsubseteq> Afix \<Gamma>\<cdot>(Aexp e\<cdot>(stack_arity S))"
+proof(cases e rule: maybeVar.cases)
+case goal1
+  have "up\<cdot>(stack_arity S) \<sqsubseteq> (Aexp (Var x)\<cdot>(stack_arity S)) x" by (simp add: Aexp_Var)
+  also have "(Aexp (Var x)\<cdot>(stack_arity S)) \<sqsubseteq>  (Afix \<Gamma>\<cdot>(Aexp (Var x)\<cdot>(stack_arity S)))" by (rule Afix_above_arg)
+  finally
+  have "up\<cdot>(stack_arity S) \<sqsubseteq> (Afix \<Gamma>\<cdot>(Aexp (Var x)\<cdot>(stack_arity S))) x" by this simp
+  thus ?thesis using `e = _` by simp
+qed auto
+
+theorem
+  assumes "(\<Gamma>, e, S) \<Rightarrow>\<^sup>*\<^bsub>T\<^esub> final"
+  shows "trace_arities ((\<Gamma>, e, S) # T) \<sqsubseteq> Afix \<Gamma> \<cdot> (Aexp e \<cdot> (stack_arity S))"
+using assms
+proof(induction rule: conf_trace_induct_final)
+  case (trace_nil \<Gamma> e S)
+    thus ?case by (simp del: app_strict conf_arities.simps) (rule arity_correct_now)
+next
+  case (trace_cons \<Gamma> e S T \<Gamma>' e' S')
+
+  have "conf_arities (\<Gamma>, e, S) \<sqsubseteq> Afix \<Gamma>\<cdot>(Aexp e\<cdot>(stack_arity S))" by (rule arity_correct_now)
+  moreover
+  note `trace_arities ((\<Gamma>', e', S') # T) \<sqsubseteq> Afix \<Gamma>'\<cdot>(Aexp e'\<cdot>(stack_arity S'))`
+  moreover
+  from `(\<Gamma>, e, S) \<Rightarrow> (\<Gamma>', e', S')`
+  have "Afix \<Gamma>'\<cdot>(Aexp e'\<cdot>(stack_arity S')) \<sqsubseteq> Afix \<Gamma>\<cdot>(Aexp e\<cdot>(stack_arity S))"
+    by (rule arity_preservation)
+  ultimately
+  show ?case by (auto intro: join_below dest: below_trans simp del: conf_arities.simps fun_meet_simp)
+qed
+
+end
